---
layout: post
title: U3 Hacks
comments: true
courses: { csa: {week: 8} }
type: hacks
---

# Your Homework

Now that you know what boolean expressions are and how to write them, as well as several comparison methods, your task is to write a class that uses either the compareTo or comparator and compare. Then create two instances of these classes and demonstrate using if statements.

BONUS: Create a program that checks if a year is a leap year or not.

Here is how the method should work:

(1) Prompt the user to input any year that they would like <br>
(2) Determine if the year is a leap year or not <br>
(3) Print the necessary dialogue (ex. [year] is/is not a leap year) AND return the value of any boolean(s) used

```java
import java.util.Scanner;

public class LeapYearChecker {

    public static void main(String[] args) {
        Scanner scanner = new Scanner(System.in);

        System.out.print("Enter a year: ");
        int year = scanner.nextInt();
        boolean isLeapYear = isLeapYear(year);

        System.out.println(year + (isLeapYear ? " is a leap year." : " is not a leap year."));
    }

    public static boolean isLeapYear(int year) {
        if ((year % 4 == 0 && year % 100 != 0) || (year % 400 == 0)) {
            return true;
        } else {
            return false;
        }
    }
}
java
Copy code
// Demo
public class Demo {
    public static void main(String[] args) {
        LeapYearChecker year1 = new LeapYearChecker(2007);
        LeapYearChecker year2 = new LeapYearChecker(2020);

        boolean isLeap1 = year1.isLeapYear();
        boolean isLeap2 = year2.isLeapYear();

        System.out.println("2007 is a leap year: " + isLeap1);
        System.out.println("2020 is a leap year: " + isLeap2);
    }
}

Demo.main(null);
Weird questions
!(true)&&(false) = ? what in boolean values?

!(true)&&(false) = false && false = false

not ((((true and not (false)) ^ false) ^ true) && false) (remember PEMDASNAO!)

not ((((true and not (false)) ^ false) ^ true) && false) = not (((true ^ false) ^ true) && false) = not ((true ^ true) && false) = not (true && false) = not false = true

Prove the following: !A * !(B + !C) = !A * (!B * !C)

!A * (!B * C) = !A * (!C * !B)

Using the law of association, !C * !B = !B * !C

Therefore, !A * (!B * C) = !A * (!C * !B) = !A * (!B * !C)

420 && 66 (Hint, convert to binary, then perform the operation)

420 --> 110100100
66 --> 001000010 (assuming the same number of digits as 420)

110100100 & 001000010 --> 000000000 => 0

If you got this one, try 89 OR 42

89 = 1011001 in binary
42 = 0101010 in binary (assuming the same number of digits as 89)

1011001 & 0101010 --> 1111011 => 123
